src/TwoDisk/AsyncTwoDiskAPI.v
@@ -1,7 +1,7 @@
 Require Import Prog.
 Require Import Automation.
 
-Require Import Disk.SimpleDisk.
+Require Import Disk.AsyncDisk.
 Require Export TwoDisk.TwoDiskDefs.
 Require Import Refinement.Interface.
 
@@ -9,17 +9,21 @@ Module TD.
 
   Import TwoDiskDefs.TD.
 
-  (* shadow state with a specialized version for sequential disks *)
+  (* shadow state with a specialized version for async disks *)
   Definition State := TD.State disk.
 
   (* help out type inference *)
   Implicit Type (state:State).
 
+  Definition bg_step state state'' :=
+    exists state', bg_failure state state' /\
+          disks_rel pflushed state state'.
+
   Inductive op_step : forall `(op: Op T), Semantics State T :=
   | step_read : forall a i r state,
       match get_disk i state with
       | Some d => match d a with
-                 | Some b0 => r = Working b0
+                 | Some b0 => r = Working (latest b0)
                  | None => exists b, r = Working b
                  end
       | None => r = Failed
@@ -27,15 +31,20 @@ Module TD.
       op_step (Read i a) state r state
   | step_write : forall a i b state r state',
       match get_disk i state with
-      | Some d => state' = set_disk i state (diskUpd d a b) /\
+      | Some d => match d a with
+                 | Some bs0 => state' = set_disk i state (diskUpd d a (buffer b bs0))
+                 | None => state' = state
+                 end /\
                  r = Working tt
       | None => r = Failed /\ state' = state
       end ->
       op_step (Write i a b) state r state'
   | step_sync : forall i state r state',
       match get_disk i state with
-      | Some d => state' = state /\ r = Working tt
-      | None => r = Failed /\ state' = state
+      | Some d => state' = set_disk i state (flush d) /\
+                 r = Working tt
+      | None => state' = state /\
+               r = Failed
       end ->
       op_step (Sync i) state r state'
   | step_size : forall i state r,
@@ -48,7 +57,7 @@ Module TD.
   Definition wipe state := state.
 
   Definition API : InterfaceAPI Op State :=
-    background_step bg_failure (@op_step) wipe.
+    background_step bg_step (@op_step) wipe.
 
   Ltac inv_step :=
     match goal with
@@ -56,12 +65,6 @@ Module TD.
       inversion H; subst; clear H;
       repeat sigT_eq;
       safe_intuition
-    end.
-
-  Ltac inv_bg :=
-    match goal with
-    | [ H: bg_failure _ _ |- _ ] =>
-      inversion H; subst; clear H
     end.
 
 End TD.
